theories/EagerContract.v
@@ -1,0 +1,106 @@
+Require Import CSL.Contract.
+Require Import Lists.List.
+Import ListNotations.
+
+Inductive Tau : Contract -> Contract -> Prop :=
+ | TPlusL c c' : Tau (c _+_ c') c
+ | TPlusR c c' : Tau (c _+_ c') c'
+ | TSeqSuc c : Tau (Success _;_ c) c
+ | TSeqStep c c0 c1 (H0: Tau c0 c1): Tau (c0 _;_ c) (c1 _;_ c).
+Hint Constructors Tau : core.
+
+
+Inductive EDerive : Contract -> EventType -> Contract -> Prop :=
+ | ESuccess e : EDerive Success e Failure
+ | EFailure e : EDerive Failure e Failure
+ | EEventS e : EDerive (Event e) e Success
+ | EEventF e0 e (H0: e0 <> e) : EDerive (Event e0) e Failure
+ | ESeqStep e c c0 c1 (H0: EDerive c0 e c1): EDerive (c0 _;_ c) e (c1 _;_ c)
+ | ETauStep e c0 c0' c1 (H0: Tau c0 c0') (H1: EDerive c0' e c1) : EDerive c0 e c1.
+Hint Constructors EDerive : core.
+
+Lemma Tau_soundness : forall (c0 c1 : Contract), Tau c0 c1 -> (forall s, s ==~ c1 -> s ==~ c0).
+Proof.
+intros. generalize dependent s. induction H;intros;auto.
+- rewrite <- (app_nil_l s). auto. 
+- inversion H0. constructor; auto.
+Qed.
+
+Lemma EDerive_soundness : forall (c0 c1 : Contract)(e : EventType), EDerive c0 e c1 -> (forall s, s ==~ c1 -> s ==~ c0 / e).
+Proof.
+intros. generalize dependent s. induction H;intros;simpl;try solve [inversion H0].
+- destruct (eq_event_dec e e). auto. contradiction.
+- inversion H1.
+- destruct (nu c0) eqn:Heqn.
+  * inversion H0. apply MPlusL. constructor;auto. 
+  * inversion H0.  constructor;auto. 
+- apply IHEDerive in H1. rewrite <- derive_spec_comp. rewrite <- derive_spec_comp in H1.
+  apply (Tau_soundness _ _ H0). assumption.
+Qed.
+
+Ltac rewrite_forall l := exists l; split; try (rewrite Forall_forall; intros; inversion H; subst; auto; inversion H0).
+
+Inductive TauSteps : Contract -> Contract -> Prop :=
+ | TauNone c : TauSteps c c
+ | TauMore c0 c1 c2 (H0: Tau c0 c1) (H1:TauSteps c1 c2) : TauSteps c0 c2.
+Hint Constructors TauSteps : core.
+
+Lemma TauStepsSeq : forall (c0 c1 c : Contract), TauSteps c0 c1 -> TauSteps (c0 _;_ c) (c1 _;_ c).
+Proof.
+intros. generalize dependent c. induction H;intros.
+- constructor.
+- apply TauMore with (c1 _;_ c);eauto.
+Qed.
+
+Lemma TauStepTrans : forall (c0 c1 c2 : Contract), TauSteps c0 c1 -> TauSteps c1 c2 -> TauSteps c0 c2.
+Proof. intros. generalize dependent c2. induction H;intros;eauto. Qed.
+
+
+Lemma TauSteps_Nu : forall (c : Contract), Nu c -> TauSteps c Success.
+Proof. intros. induction H;intros;eauto. apply TauStepTrans with (Success _;_ c1);eauto using TauStepsSeq. Qed.
+
+
+Lemma TauSteps_EDerive : forall (c0 c1 c2 : Contract)(e : EventType), TauSteps c0 c1 -> EDerive c1 e c2 -> EDerive c0 e c2.
+Proof. intros. induction H.
+- assumption.
+- apply ETauStep with c1;auto.
+Qed.
+
+Lemma EDerive_completeness : forall (c c' : Contract)(e : EventType), Derive c e c' -> exists (l : list Contract), 
+Forall (EDerive c e) l /\ (forall s, s ==~ c'-> s ==~ plus_fold l).
+Proof.
+intros. induction H.
+- rewrite_forall [Failure]. intros. inversion H.
+- rewrite_forall [Failure]. intros. inversion H.
+- rewrite_forall [Success]. intros. inversion H. simpl. auto.
+- rewrite_forall [Failure]. rewrite Forall_forall. intros. inversion H. subst. auto. inversion H1.
+  intros. inversion H. 
+- destruct IHDerive1 as [l1 [P1 P2]]. destruct IHDerive2 as [l2 [P3 P4]].
+   exists (l1++l2). split.
+  * rewrite Forall_forall in *. intros. apply in_app_or in H1 as [H1 | H1].
+    ** eapply ETauStep. eapply TPlusL. eauto.
+    ** eapply ETauStep. eapply TPlusR. eauto.
+  * intros. rewrite plus_fold_app. inversion H1;auto.
+- destruct IHDerive1 as [l1 [P1 P2]]. destruct IHDerive2 as [l2 [P3 P4]].
+  exists (l2 ++ (map (fun c => c _;_ c1) l1)). split.
+  * rewrite Forall_forall. intros. apply in_app_or in H2 as [H2 | H2].
+    ** rewrite Forall_forall in P3. apply TauSteps_Nu in H0. apply TauSteps_EDerive with (Success _;_ c1). 
+      *** apply TauStepsSeq. assumption.
+      *** eauto.
+    ** rewrite in_map_iff in H2. destruct H2 as [c [P5 P6]].
+       subst. constructor. rewrite Forall_forall in P1. auto.
+  * intros. rewrite plus_fold_app. inversion H2;subst.
+    ** inversion H5. subst. apply MPlusR. apply P2 in H7. rewrite in_plus_fold in H7.
+       destruct H7 as [c' [P9 P10]]. rewrite in_plus_fold. exists (c' _;_ c1). split.
+      *** rewrite in_map_iff. exists c'. split. reflexivity. assumption.
+      *** auto.
+    ** apply MPlusL. auto.
+- destruct IHDerive as [l [P1 P2]]. exists (map (fun c => c _;_ c1) l). split.
+  * rewrite Forall_forall in *. intros. rewrite in_map_iff in H1.
+    destruct H1 as [c' [P3 P4]]. subst. auto.
+  * intros. inversion H1. subst. rewrite in_plus_fold.
+    apply P2 in H5. rewrite in_plus_fold in H5. destruct H5 as [c' [P3 P4]].
+    exists (c' _;_ c1). rewrite in_map_iff. split.
+    ** exists c'. split. reflexivity. assumption.
+    ** auto.
+Qed.
